Implemented carrying, which requires defining over Z rather than arbitrary ring

src/NewBaseSystem.v
@@ -3,120 +3,43 @@ Require Import Crypto.Util.Decidable.
 Require Import Coq.Lists.List.
 Require Import Crypto.Algebra. Import Ring.
 Require Import Coq.ZArith.BinInt.
+Require Import Coq.ZArith.ZArith.
+Local Open Scope Z_scope.
 
 Module B.
   Section NewBaseSystem.
-    Context {R Req Rzero Rone Ropp Radd Rmul Rsub}
-            {ZRmul : Z -> R -> R} {ZRmul_0_r:forall b, ZRmul b Rzero = Rzero}
-            {ZRmul_Zmul_Rmul : forall x y a b, ZRmul (x * y)%Z (Rmul a b) = Rmul (ZRmul x a) (ZRmul y b)}
-            {ZRmul_distr_add_l : forall x a b, ZRmul x (Radd a b) = Radd (ZRmul x a) (ZRmul x b)}
-            {ZRmul_ZRmul : forall x y a, ZRmul x (ZRmul y a) = ZRmul (x * y)%Z a}
-            {Rring:@Algebra.ring R Req Rzero Rone Ropp Radd Rsub Rmul}.
-    Local Infix "=" := Req : type_scope.
-    Local Infix "*" := Rmul.
-    Local Infix "+" := Radd.
+    Let rep : Type := list (Z * Z).
 
-    Let coef := Z.
-    Let rep : Type := list (coef * R).
+    Definition eval (p:rep) : Z :=
+      fold_right Z.add 0 (map (fun t => (fst t) * (snd t)) p).
 
-    Definition evalterm (t:coef*R) : R :=
-      let '(c, x) := t in ZRmul c x.
-
-    Definition eval (p:rep) : R :=
-      fold_right Radd Rzero (map evalterm p).
-
-    Lemma eval_nil : eval nil = Rzero. Proof. reflexivity. Qed.
-    Lemma eval_cons p q : eval (p::q) = evalterm p + eval q. Proof. reflexivity. Qed.
-    Lemma eval_app p q: eval (p++q) = eval p + eval q.
-    Proof.
-      induction p; intros; [rewrite ?app_nil_l, ?eval_nil, ?left_identity; reflexivity|].
-      rewrite <-!app_comm_cons, !eval_cons, IHp; auto using associative.
-    Qed.
+    Definition add (p q : rep) : rep := p ++ q.
 
     Definition mul (p q:rep) : rep :=
       flat_map (fun t => let '(c, x) := t in
                          map (fun t' => let '(c', x') := t' in
-                                        (Z.mul c c', Rmul x x')) q) p.
+                                        (c * c', x * x')) q) p.
 
-    Lemma mul_single a q : eval (mul (a :: nil) q) = evalterm a * eval q.
-    Proof.
-      induction q; intros; simpl mul; destruct_head prod;
-        rewrite ?eval_nil, ?eval_cons, ?app_nil_r, ?mul_0_r in *; try reflexivity.
-      match goal with |- eval (?x :: ?y) = _ => rewrite (eval_cons x y) end.
-      simpl evalterm; rewrite IHq, left_distributive, ZRmul_Zmul_Rmul. reflexivity.
-    Qed.
-    
-    Lemma mul_correct' a p q :
-      eval (mul (a :: p) q) = eval (mul (a :: nil) q) + eval (mul p q).
-    Proof.
-      intros; simpl mul; rewrite ?eval_nil, ?eval_cons, ?app_nil_r, <-?eval_app. reflexivity.
-    Qed.
-
-    Lemma mul_correct p q : eval (mul p q) = Rmul (eval p) (eval q).
-    Proof.
-      induction p; [destruct q; simpl; rewrite ?eval_nil, ?mul_0_l; reflexivity |].
-      rewrite mul_correct', mul_single, eval_cons, IHp, right_distributive; reflexivity.
-    Qed.
-
-    Definition add (p q : rep) : rep := p ++ q.
-
-    Lemma add_correct p q : eval (add p q) = Radd (eval p) (eval q).
-    Proof.
-      induction p; simpl; rewrite ?eval_nil, ?eval_cons, ?left_identity, ?IHp, ?associative; reflexivity.
-    Qed.
-
-    Definition gather_or_leave b cx gso : rep * R :=
+    Definition gather_or_leave b cx gso : rep * Z :=
       if dec (Logic.eq ((fst cx) mod b) 0)%Z
-      then (fst gso, ZRmul ((fst cx) / b) (snd cx) + snd gso) (* TODO: use a compile-time scaling operation that compile-time checks whether the coefficient is 1 and skips multiplication if so. Maybe use notation scopes for compiletime and runtime. *)
+      then (fst gso, Z.add (((fst cx) / b) * (snd cx)) (snd gso)) (* TODO: use a compile-time scaling operation that compile-time checks whether the coefficient is 1 and skips multiplication if so. Maybe use notation scopes for compiletime and runtime. *)
       else (cx :: fst gso, snd gso).
 
-    Definition gather_single (b : Z) (p : rep) : rep * R :=
-      fold_right (gather_or_leave b) (nil,Rzero) p.
+    Definition gather_single (b : Z) (p : rep) : rep * Z :=
+      fold_right (gather_or_leave b) (nil,0) p.
 
-    Definition gather' (base:list Z) (p:rep) : (rep * list R) :=
+    Definition gather' (base:list Z) (p:rep) : (rep * list Z) :=
       fold_right (fun b state =>
                     let gso := gather_single b (fst state) in
                     (fst gso, snd gso::snd state)) (p, nil) base.
     Definition gather b p := snd (gather' b p).
 
-    Lemma gather_single_all p : Logic.eq (fst (gather_single 1%Z p)) nil.
-    Proof.
-      induction p; [solve [trivial]|]; simpl gather_single.
-      unfold gather_or_leave; rewrite Z.mod_1_r, IHp.
-      break_match; [reflexivity|congruence].
-    Qed.
-
-    Lemma gather_all base' p : Logic.eq (fst (gather' (1%Z::base') p)) nil.
-    Proof. unfold gather'; simpl fst; setoid_rewrite gather_single_all; reflexivity. Qed.
-
-    Lemma gather_single_correct b (b_nonzero : b <> 0%Z) p :
-      Radd (eval (fst (gather_single b p))) (ZRmul b (snd (gather_single b p))) = eval p.
-    Proof.
-      induction p; simpl; [rewrite ?eval_nil, ?left_identity, ?ZRmul_0_r;reflexivity|].
-      cbv [gather_or_leave]; destruct_head' prod; break_match; try congruence; simpl;
-        rewrite !eval_cons; simpl; rewrite <-IHp; simpl fst in *.
-      { rewrite ZRmul_distr_add_l, ZRmul_ZRmul, <-Zdiv.Z_div_exact_full_2 by auto.
-        rewrite !associative; apply Group.cancel_right, commutative. }
-      { setoid_rewrite eval_cons; rewrite associative; reflexivity. }
-    Qed.
-
-    Lemma gather'_correct base : forall p, (forall b, In b base -> b <> 0%Z) ->
-      eval (fst (gather' base p)) + eval (combine base (snd (gather' base p))) = eval p.
-    Proof.
-      induction base; intros; simpl; [rewrite eval_nil; auto using right_identity|].
-      setoid_rewrite eval_cons; cbv [evalterm]; rewrite associative.
-      rewrite gather_single_correct; auto using in_cons, in_eq.
-    Qed.
-
-    Lemma gather_correct base p : (forall b, In b base -> b <> 0%Z) ->
-      eval (combine (1%Z::base) (gather (1%Z::base) p)) = eval p.
-    Proof.
-      intros. etransitivity; [|eapply gather'_correct; eassumption].
-      simpl; setoid_rewrite eval_cons; cbv [evalterm].
-      rewrite <-gather_single_correct with (p := fst (gather' base p)) (b := 1%Z) by congruence.
-      rewrite gather_single_all, eval_nil, left_identity.
-      reflexivity.
-    Qed.
+    Definition carry (from next : Z) (p : rep) : rep :=
+      let cap := (next / from)%Z in
+      flat_map (fun cx => let '(c,x) := cx in
+                          if dec (Logic.eq c from)
+                          then ((c, x mod cap) :: (next, x / cap) :: nil)%Z
+                          else nil) p.
 
   (*
     Let base := (1::10::100::1000::10000::100000::1000000::10000000::nil)%Z.
@@ -132,4 +55,76 @@ Module B.
     Compute gather base (mul f g).
   *)
 
-End NewBaseSystem.
+    Section NewBaseSystemProofs.
+
+    Lemma eval_nil : eval nil = 0. Proof. reflexivity. Qed.
+    Lemma eval_cons p q : eval (p::q) = (fst p) * (snd p) + eval q. Proof. reflexivity. Qed.
+    Lemma eval_app p q: eval (p++q) = eval p + eval q.
+    Proof.
+      induction p; intros; [rewrite ?app_nil_l, ?eval_nil, ?left_identity; reflexivity|].
+      rewrite <-!app_comm_cons, !eval_cons, IHp; auto using associative.
+    Qed.
+    
+    Lemma add_correct p q : eval (add p q) = eval p + eval q.
+    Proof.
+      induction p; simpl; rewrite ?eval_nil, ?eval_cons, ?left_identity, ?IHp, ?associative; reflexivity.
+    Qed.
+
+    Lemma mul_single a q : eval (mul (a :: nil) q) = fst a * snd a * eval q.
+    Proof.
+      induction q; intros; simpl mul; destruct_head prod;
+        rewrite ?eval_nil, ?eval_cons, ?app_nil_r, ?mul_0_r in *; try reflexivity.
+      simpl. rewrite IHq, left_distributive. ring. 
+    Qed.
+    
+    Lemma mul_correct' a p q :
+      eval (mul (a :: p) q) = eval (mul (a :: nil) q) + eval (mul p q).
+    Proof.
+      intros; simpl mul; rewrite ?eval_nil, ?eval_cons, ?app_nil_r, <-?eval_app. reflexivity.
+    Qed.
+
+    Lemma mul_correct p q : eval (mul p q) = eval p * eval q.
+    Proof.
+      induction p; [destruct q; simpl; rewrite ?eval_nil, ?mul_0_l; reflexivity |].
+      rewrite mul_correct', mul_single, eval_cons, IHp; ring.
+    Qed.
+
+    Lemma gather_single_all p : Logic.eq (fst (gather_single 1%Z p)) nil.
+    Proof.
+      induction p; [solve [trivial]|]; simpl gather_single.
+      unfold gather_or_leave; rewrite Z.mod_1_r, IHp.
+      break_match; [reflexivity|congruence].
+    Qed.
+
+    Lemma gather_all base' p : Logic.eq (fst (gather' (1%Z::base') p)) nil.
+    Proof. unfold gather'; simpl fst; setoid_rewrite gather_single_all; reflexivity. Qed.
+
+    Lemma gather_single_correct b (b_nonzero : b <> 0%Z) p :
+      eval (fst (gather_single b p)) + (b * snd (gather_single b p)) = eval p.
+    Proof.
+      induction p; simpl; [rewrite ?eval_nil; ring|].
+      cbv [gather_or_leave]; destruct_head' prod; break_match; try congruence; simpl;
+        rewrite !eval_cons; simpl; rewrite <-IHp; simpl fst in *; [|ring].
+      rewrite Z.mul_add_distr_l, !Z.mul_assoc, <-Zdiv.Z_div_exact_full_2;
+        auto; ring.
+    Qed.
+
+    Lemma gather'_correct base : forall p, (forall b, In b base -> b <> 0%Z) ->
+      eval (fst (gather' base p)) + eval (combine base (snd (gather' base p))) = eval p.
+    Proof.
+      induction base; intros; simpl; [rewrite eval_nil; auto using right_identity|].
+      setoid_rewrite eval_cons. rewrite associative, gather_single_correct; auto using in_cons, in_eq.
+    Qed.
+
+    Lemma gather_correct base p : (forall b, In b base -> b <> 0%Z) ->
+      eval (combine (1%Z::base) (gather (1%Z::base) p)) = eval p.
+    Proof.
+      intros. etransitivity; [|eapply gather'_correct; eassumption].
+      simpl; setoid_rewrite eval_cons.
+      rewrite <-gather_single_correct with (p := fst (gather' base p)) (b := 1%Z) by congruence.
+      rewrite gather_single_all, eval_nil. simpl fst; simpl snd. ring.
+    Qed.
+
+    End NewBaseSystemProofs.
+  End NewBaseSystem.
+End B.
